Add hash trait example

CoqOfRust/CoqOfRust.v
@@ -59,7 +59,7 @@ Export M.Notations.
     for now. It will drive the monadic transformation in near future. *)
 Notation "e (| e1 , .. , en |)" :=
   ((.. (e e1) ..) en)
-  (at level 0, 
+  (at level 0,
     only parsing).
 
 (** Particular case when there are no arguments. *)
@@ -114,6 +114,9 @@ Parameter cast : forall {A : Set}, A -> forall (B : Set), B.
 
 Parameter assign : forall {A : Set}, A -> A -> M unit.
 
+Definition usize : Set := Z.
+Definition isize : Set := Z.
+
 Definition u8 : Set := Z.
 Definition u16 : Set := Z.
 Definition u32 : Set := Z.
@@ -157,6 +160,8 @@ Global Instance Method_destroy (A : Set) : Notation.Dot "destroy" := {
   Notation.dot (x : A) := Pure tt;
 }.
 
+Global Instance Method_ne_u64 : Notation.Dot "ne" (T := u64 -> u64 -> M bool). Admitted.
+
 Module Root.
   Module std.
     Module prelude.
@@ -167,7 +172,21 @@ Module Root.
 End Root.
 
 Module std.
-  Module string.
+  Module collections.
+   Module hash_map.
+     Module DefaultHasher.
+       Parameter t : Set.
+       Definition new (_ : unit) : M t. Admitted.
+
+       Global Instance DefaultHasher_new : Notation.DoubleColon t "new" := {
+         Notation.double_colon := new
+       }.
+     End DefaultHasher.
+     Definition DefaultHasher := DefaultHasher.t.
+   End hash_map.
+  End collections.
+
+ Module string.
     Module ToString.
       Class Trait (Self : Set) : Set := {
         to_string : ref Self -> M String;
@@ -403,6 +422,121 @@ Module std.
     Global Instance Write_for_Formatter : Write.Trait Formatter.
     Admitted.
   End fmt.
+
+  (* @TODO: There is a module [std.hash] in [std/hash.v] which was
+     added with the remaining of the stdlib, the module below
+     was added alone to make trait.rs example work, they differ
+     slightly, TODO: we should have only one of them *)
+  Module hash.
+    Module BuilHasherDefault.
+      Record t (H : Set) : Set := { }.
+    End BuilHasherDefault.
+    Definition BuilHasherDefault := BuilHasherDefault.t.
+
+    Module Hasher.
+      Class Trait (Self : Set) : Set := {
+      (* fn finish(&self) -> u64; *)
+      finish : ref Self -> M u64;
+
+      (* fn write(&mut self, bytes: &[u8]); *)
+      write : mut_ref Self -> ref (list u8) -> unit;
+
+      (* fn write_u8(&mut self, i: u8) { ... } *)
+      write_u8 : mut_ref Self -> u8 -> unit;
+
+      (* fn write_u16(&mut self, i: u16) { ... } *)
+      write_u16 : mut_ref Self -> u16 -> unit;
+
+      (* fn write_u32(&mut self, i: u32) { ... } *)
+      write_u32 : mut_ref Self -> u32 -> unit;
+
+      (* fn write_u64(&mut self, i: u64) { ... } *)
+      write_u64 : mut_ref Self -> u64 -> unit;
+
+      (* fn write_u128(&mut self, i: u128) { ... } *)
+      write_u128 : mut_ref Self -> u128 -> unit;
+
+      (* fn write_usize(&mut self, i: usize) { ... } *)
+      write_usize : mut_ref Self -> usize -> unit;
+
+      (* fn write_i8(&mut self, i: i8) { ... } *)
+      write_i8 : mut_ref Self -> i8 -> unit;
+
+      (* fn write_i16(&mut self, i: i16) { ... } *)
+      write_i16 : mut_ref Self -> i16 -> unit;
+
+      (* fn write_i32(&mut self, i: i32) { ... } *)
+      write_i32 : mut_ref Self -> i32 -> unit;
+
+      (* fn write_i64(&mut self, i: i64) { ... } *)
+      write_i64 : mut_ref Self -> i64 -> unit;
+
+      (* fn write_i128(&mut self, i: i128) { ... } *)
+      write_i128 : mut_ref Self -> i128 -> unit;
+
+      (* fn write_isize(&mut self, i: isize) { ... } *)
+      write_isize : mut_ref Self -> isize -> unit;
+
+      (* fn write_length_prefix(&mut self, len: usize) { ... } *)
+      write_length_prefix : mut_ref Self -> usize -> unit;
+
+      (* fn write_str(&mut self, s: &str) { ... } *)
+      write_str : mut_ref Self -> ref str;
+      }.
+    End Hasher.
+
+    Module Hash.
+      Class Trait (Self : Set) : Set := {
+        hash {H : Set}
+          `{Hasher : Hasher.Trait H}
+          : ref Self -> mut_ref H -> M unit;
+
+          
+        (* @TODO 
+        hash_slice (H : Set)
+          `{Hasher.Trait H}
+          (* `{Sized.Trait Self} *)
+          : ref (list Self) -> M (mut_ref H);
+         *)
+      }.
+    End Hash.
+
+    Module BuildHasher.
+      Class Trait (Self Hasher : Set)
+        `{Hasher.Trait Hasher}
+        : Set := {
+          Hasher := Hasher;
+          build_hasher : ref Self -> Hasher;
+          hash_one (T : Set)
+            `{Hash.Trait T}
+            (* `{Sized.Trait Self} *)
+            `{Hasher.Trait Hasher}
+            : ref Self -> T -> u64;
+      }.
+    End BuildHasher.
+
+    (** Hasher instance functions *)
+    Global Instance Hasher_Method_finish (T : Set) `{Hasher.Trait T} : Notation.Dot "finish" := {
+      Notation.dot (x : T) := Hasher.finish x;
+    }.
+
+    (** Hash instance functions *)
+    Global Instance Hash_Method_hash (T : Set) `{Hasher.Trait} `{Hash.Trait T} : Notation.Dot "hash" := {
+        Notation.dot (x : T) := Hash.hash x;
+    }.
+
+    (** Hasher implementation for DefaultHasher *)
+    Global Instance DefaultHasher_Hasher : Hasher.Trait std.collections.hash_map.DefaultHasher. Admitted.
+
+    (** Hash implementation for primitive types *)
+    Global Instance Hash_for_unit : Hash.Trait unit. Admitted.
+    Global Instance Hash_for_bool : Hash.Trait unit. Admitted.
+    Global Instance Hash_for_i32 : Hash.Trait i32. Admitted.
+    Global Instance Hash_for_u32 : Hash.Trait u32. Admitted.
+    Global Instance Hash_for_String : Hash.Trait String. Admitted.
+    Global Instance Hash_for_i64 : Hash.Trait i64. Admitted.
+    Global Instance Hash_for_u64 : Hash.Trait u64. Admitted.
+  End hash.
 
   Module prelude.
     Module rust_2021.
@@ -863,10 +997,10 @@ Module std.
         ne : ref Self -> ref Rhs -> M bool;
       }.
 
-      Global Instance Method_eq `(Trait) : Notation.Dot "eq" := { 
+      Global Instance Method_eq `(Trait) : Notation.Dot "eq" := {
         Notation.dot := eq;
       }.
-      Global Instance Method_ne `(Trait) : Notation.Dot "ne" := { 
+      Global Instance Method_ne `(Trait) : Notation.Dot "ne" := {
         Notation.dot := ne;
       }.
     End PartialEq.
@@ -882,19 +1016,19 @@ Module std.
         ge : ref Self -> ref Rhs -> M bool;
       }.
 
-      Global Instance Method_partial_cmp `(Trait) : Notation.Dot "partial_cmp" := { 
+      Global Instance Method_partial_cmp `(Trait) : Notation.Dot "partial_cmp" := {
         Notation.dot := partial_cmp;
       }.
-      Global Instance Method_lt `(Trait) : Notation.Dot "lt" := { 
+      Global Instance Method_lt `(Trait) : Notation.Dot "lt" := {
         Notation.dot := lt;
       }.
-      Global Instance Method_le `(Trait) : Notation.Dot "le" := { 
+      Global Instance Method_le `(Trait) : Notation.Dot "le" := {
         Notation.dot := le;
       }.
-      Global Instance Method_gt `(Trait) : Notation.Dot "gt" := { 
+      Global Instance Method_gt `(Trait) : Notation.Dot "gt" := {
         Notation.dot := gt;
       }.
-      Global Instance Method_ge `(Trait) : Notation.Dot "ge" := { 
+      Global Instance Method_ge `(Trait) : Notation.Dot "ge" := {
         Notation.dot := ge;
       }.
     End PartialOrd.
@@ -1119,9 +1253,15 @@ Module _crate.
 
   Module fmt := std.fmt.
 
+  Module hash := std.hash.
+
   Module log.
     Parameter sol_log : str -> M unit.
   End log.
+
+  Module panicking.
+    Parameter panic : String -> M unit.
+  End panicking.
 End _crate.
 
 Module num_derive.
@@ -1213,4 +1353,3 @@ Definition format_argument : Set := std.fmt.ArgumentV1.
 
 (** A LangItem generated by the Rust compiler. *)
 Definition format_arguments : Set := std.fmt.Arguments.
-
